\documentclass{article}
\usepackage[utf8]{inputenc}
\usepackage{xcolor}

\title{Differential and Integral Calculus - Exercises}
\author{Author}
\date{October 2022 - February 2023}

\begin{document}

\maketitle

\subsection{Some rules and relevant algebra}
Rewriting roots as rational exponents

$
\\
\sqrt{x} = x^{\frac{1}{2}}
\\
\\
\frac{1}{\sqrt{x}} = x^{-\frac{1}{2}}
\\
\\
(\sqrt{x})' = \frac{1}{2\sqrt{x}} = \frac{1}{2}x^{-\frac{1}{2}}
$

\subsection{Graphs}
Things to do:
\\
1. Determine the domain of the function.
\\
2. Determine the zero points of the function. ($f(x) = 0$)
\\
3. Determine whether the function is even or odd or neither.
\\
$f(-x) = f(x)$ | EVEN
\\
$f(-x) = -f(x)$ | ODD
\\
4. Find the stationary points, 1st level (first derivative)
\\
5. Find the stationary points, 2nd level (second derivative)
\\
6. Find the asymptotes

\pagebreak

\section{Simple derivatives}

\subsection{Mini test: $f(x) = \frac{x^5}{e^x}$ (using quotient rule)}
$
  f'(x) = \frac{(x^5)' \cdot e^x - x^5 \cdot (e^x)'}{(e^x)^2}
  \\
  \\
  f'(x) = \frac{5x^4 \cdot e^x - x^5 \cdot e^x}{e^{2x}}
  \\
  \\
  f'(x) = \frac{e^x (5x^4 - x^5)}{e^{2x}}
  \\
  \\
  f'(x) = \frac{5x^4 - x^5}{e^x}
$

\subsection{a) $f(x) = x^3 + 5x + 7$}
$
f'(x) = 3x^2 + 5 + 0
\\
\\
f'(x) = 3x^2 + 5
$

\subsection{b) $f(x) = (x+5)(x-4)$}
$
f'(x) = (x+5) \cdot (x-4)
\\
\\
f'(x) = (x+5)' \cdot (x-4) + (x+5) \cdot (x-4)'
\\
\\
f'(x) = 1 \cdot (x-4) + (x+5) \cdot 1
\\
\\
f'(x) = 2x + 1
$

\subsection{c) $f(x) = (x+5)^2(x-4)$}
$
f'(x) = ((x+5)^2)' \cdot (x-4) + (x+5)^2 \cdot (x-4)'
\\
\\
f'(x) = 2(x+5) \cdot (x-4) + (x+5)^2 \cdot 1
\\
\\
f'(x) = 2x^2 - 4x + 5x - 20 + x^2 + 25
\\
\\
f'(x) = 3x^2 + x + 5
$

\pagebreak

\subsection{d) $f(x) = \frac{x}{e} + \pi $}
$
f'(x) = (\frac{x}{e})' + 0
\\
\\
f'(x) = \frac{(x)' \cdot e - x \cdot (e)'}{(e)^2}
\\
\\
f'(x) = \frac{1 \cdot e - x \cdot 0}{e^2}
\\
\\
f'(x) = \frac{e}{e^2}
\\
\\
f'(x) = - \frac{1}{e}
$

\subsection{e) $f(x) = \sqrt{x} + \frac{1}{\sqrt{x}}$}
$
f'(x) = (x^{\frac{1}{2}})' + (x^{-\frac{1}{2}})'
\\
\\
f'(x) = (\frac{1}{2}x^{\frac{1}{2}-1}) + (-\frac{1}{2}x^{-\frac{1}{2}-1})
\\
\\
f'(x) = (\frac{1}{2}x^{-\frac{1}{2}}) + (-\frac{1}{2}x^{-\frac{3}{2}})
\\
\\
f'(x) = (\frac{1}{2} \cdot \frac{1}{\sqrt{x}}) + (-\frac{1}{2} \cdot \frac{1}{x^{\frac{3}{2}}})
\\
\\
f'(x) = \frac{1}{2\sqrt{x}} - \frac{1}{2x^{\frac{3}{2}}}
\\
\\
f'(x) = \frac{1}{2\sqrt{x}} - \frac{1}{2\sqrt{x^3}}
$

\subsection{i) $f(x) = x^5 \cdot \sqrt[3]{x^4}$}
$
  \indent Solution.1
  \\
  \\
  f'(x) = 5x^4 \cdot x^\frac{4}{3} + x^5 \cdot \frac{4}{3}x^\frac{1}{3}
  \\
  \\
  f'(x) = 5x^\frac{16}{3} + \frac{4}{3}x^\frac{16}{3}
  \\
  \\
  f'(x) = \frac{19}{3}x^\frac{16}{3}
  \\
  \\
  \indent Solution.2
  \\
  \\
  f'(x) = (x^\frac{19}{3})'
  \\
  \\
  f'(x) = \frac{19}{3}x^{\frac{19}{3}-1}
  \\
  \\
  f'(x) = \frac{19}{3}x^\frac{16}{3}
$

\subsection{l) $f(x) = \frac{6cosx}{11sinx + x}$}
$
  f'(x) = \frac{-6sinx \cdot (11sinx + x) - 6cosx \cdot (11cosx + 1)}{(11sinx + x)^2}
  \\
  \\
  f'(x) = \frac{-66sin^2x - 6sin^2x - 66cos^2x - 6cosx}{(11sinx + x)^2}
  \\
  \\
  f'(x) = \frac{-6(11sin^2x + 11cos^2x + xsinx + cosx)}{(11sinx + x)^2}
  \\
  \\
  \color{blue}
  Pythagorean.identity: cos^2(x) + sin^2(x) = 1
  \\
  -66(cos^2x + sin^2x) = -66(1) = -66
  \color{black}
  \\
  \\
  f'(x) = \frac{-6(xsinx + cosx + 11)}{(11sinx + x)^2}
$

\subsection{o) $f(x) = \frac{x}{e^x}$}
$
  f'(x) = \frac{(x)' \cdot e^x - x \cdot (e^x)'}{(e^x)^2}
  \\
  \\
  f'(x) = \frac{1 \cdot e^x - x \cdot e^x}{(e^x)^2}
  \\
  \\
  f'(x) = \frac{(1-x) e^x}{(e^x)^2}
  \\
  \\
  f'(x) = \frac{1-x}{e^x}
$

\section{Vje≈æbe 2}




\end{document}
